

MF731

Name: Jiaze Sun

BUID: U99409081

Part 1.

(1) (a) the model:

$$S_0 \begin{cases} S_0 \cdot (1 + G_u) < S_0 \cdot (1 + G_u) \\ S_0 \cdot (1 + G_u) < S_0 \cdot (1 - G_u) \cdot (1 - G_u^u) \\ S_0 \cdot (1 - G_u) < S_0 \cdot (1 - G_u) \cdot (1 + G_u^d) \\ S_0 \cdot (1 - G_u) < S_0 \cdot (1 - G_u) \cdot (1 - G_u^d) \end{cases}$$

$$C^m(1, S_0) = k_0 S_0$$

$$\therefore k_0 S_0 = E^Q[(S_1 - S_0)^+] = \frac{1}{2} (S_0(1 + G_u) - S_0)^+ + \frac{1}{2} (S_0(1 - G_u) - S_0)^+$$

$$k_0 S_0 = \frac{1}{2} S_0 G_u$$

Similarly

$$\begin{aligned} \hat{C}^m(2) &= k_1 S_0 = E^Q[(S_2 - S_1)^+] \\ &= \frac{1}{2} \left[\frac{1}{2} (S_0(1 + G_u)(1 + G_u^u) - S_0(1 + G_u))^+ + \frac{1}{2} (S_0(1 + G_u)(1 - G_u^u) - S_0(1 + G_u))^+ \right] \\ &= \frac{1}{4} S_0 (1 + G_u) G_u^u + \frac{1}{4} S_0 (1 - G_u) G_u^d = \frac{1}{4} S_0 [(1 + 2k_0) G_u^u + (1 - 2k_0) G_u^d] \end{aligned}$$

$$\therefore G_u^u, G_u^d \text{ lie on the line, } (1 + 2k_0) G_u^u + (1 - 2k_0) G_u^d = 4k_1$$

(b) Given $X = (S_2 - S_0)^+$,

$$P_0(X) = E^{Q_0}[e^{-rT} X] = \tilde{E}^{Q_0}[X]$$

$$k_1 S_0 = E^Q[(S_1 - S_0)^+] = \frac{1}{2} S_0 G_u \quad \therefore G_u = 2k_0$$

$$C^m(2, S_0) = E^Q[(S_2 - S_1 + S_1 - S_0)^+] = (k_1 + k_0) S_0$$

$$= \frac{1}{4} [S_0(G_u + G_u^u + G_u G_u^u) + S_0(G_u - G_u^u - G_u G_u^u) + S_0(-G_u + G_u^d - G_u G_u^d) + 0]$$

$$= \begin{cases} \frac{S_0}{4} (2k_0 + (1 - 2k_0) G_u^d), & \text{if } G_u^u < \frac{2k_0}{1 + 2k_0}, G_u^d > \frac{2k_0}{1 - 2k_0} \quad ① \\ \frac{S_0}{4} \cdot 4k_0 & \text{if } G_u^u > \frac{2k_0}{1 + 2k_0}, G_u^d > \frac{2k_0}{1 - 2k_0} \quad ② \\ \frac{S_0}{4} \cdot 4k_1 & \text{if } G_u^u < \frac{2k_0}{1 + 2k_0}, G_u^d < \frac{2k_0}{1 - 2k_0} \quad ③ \\ \frac{S_0}{4} (2k_0 + (1 + 2k_0) G_u^u) & \text{if } G_u^u > \frac{2k_0}{1 + 2k_0}, G_u^d < \frac{2k_0}{1 - 2k_0} \quad ④ \end{cases}$$

$$\text{Since } 0 < k_0 < \frac{1}{2}, \quad \frac{k_0}{2} < k_1 < \min\left\{k_0, \frac{1}{4} - \frac{k_0}{2}\right\} \quad \therefore \frac{k_0}{2} < k_1 < k_0$$

$$\therefore ③ < ② < ① \text{ And } ③ < ④ < ①$$

$$M_0(X) = \begin{cases} 2k_0 + (1 - 2k_0) G_u^d - 4k_1 & \\ 2k_0 + (1 + 2k_0) G_u^u - 4k_1 & \end{cases} = \begin{cases} 2k_0 - (1 - 2k_0) G_u^u & \\ 2k_0 - (1 + 2k_0) G_u^d & \end{cases}$$

$$\therefore (4k_0, 4k_1 + 2k_0)$$

2.

a)

the empirical VaR is : 24984.392523364484

theoretical VaR is: 22773.549452807296

confidence interval for theoretical VaR: 21138.534984083803

b)

24651.99266165352

Average \bar{Y}_m : 22812.17217596515

Confidence interval: 20687.144342383945 25094.040107888293

Part 2:

1. the payoff of this defaultable ZCB under RT method is $\begin{cases} 1 & T > \tau \\ (1-\delta) & t < \tau \leq T \end{cases}$

$$\begin{aligned} \overline{ZCB}^{RT}(t, T) &= E[1_{\tau > T} e^{-\int_t^T r(u) du} + 1_{\tau \leq T} (1-\delta) e^{-\int_t^T r(u) du} | \mathcal{F}_t] \\ &= ZCB(t, T) + 1_{t < T} (1-\delta) e^{-\int_t^T r(u) du} \int_t^T r(s) e^{-\int_t^s r(u) du} ds \end{aligned}$$

$$\overline{ZCB}^{RF}(t, T) = ZCB(t, T) + 1_{\tau > T} (1-\delta) \int_t^T r(s) e^{-\int_t^s (r(u) + r(u)) du} ds$$

Assume that $r(t) \geq 0, T \leq \tau$

$$\begin{aligned} e^{-\int_t^T r(u) du} \int_t^T r(s) e^{-\int_t^s r(u) du} ds &= \int_t^T r(s) e^{-\int_t^s (r(u) + r(u)) du} e^{-\int_s^T r(u) du} ds \\ &\leq \int_t^T r(s) e^{-\int_t^s (r(u) + r(u)) du} ds \end{aligned}$$

\therefore RT gives a lower price, since RF gives a default of $(1-\delta)$ which makes the default payment higher

2.

$$\begin{aligned} \text{(a) Given } \{\tau > t\}, P_0(t, T) &= e^{-\int_t^T r(u) du} \\ P_1(t, T) &= e^{-\int_t^T (r(u) + r(u)) du} \\ P_1^{RF}(t, T) &= e^{-\int_t^T (r(u) + r(u)) du} + (1-\delta) \int_t^T r(s) e^{-\int_t^s (r(u) + r(u)) du} ds \end{aligned}$$

Then we have:

$$\begin{aligned} C(t, T) &= -\frac{1}{T-t} \left(-\int_t^T (r(u) + r(u)) du + \int_t^T r(u) du \right) = \frac{1}{T-t} \int_t^T r(u) du \\ C^{RF}(t, T) &= -\frac{1}{T-t} \log \left(e^{-\int_t^T r(u) du} + (1-\delta) \int_t^T r(s) e^{-\int_t^s (r(u) + r(u)) du} ds \right) \end{aligned}$$

$$\begin{aligned} \text{(b) By Hospital rule: } \lim_{T \rightarrow t} C(t, T) &= r(t) \\ \lim_{T \rightarrow t} C^{RF}(t, T) &= \delta r(t) \quad \text{where } \delta = 1, 0 \text{ recovery} \\ C^{RF}(t, T) &= C(t, T) \end{aligned}$$

3.

Take accrued interest into account, we have:

$$\begin{aligned} \text{premium side: } V_t^{\text{prem}}(t) &= E^Q \left[\sum_{n=1}^{NA} \frac{x}{\Delta} \cdot 1_{t_{n-1} < \tau} | \mathcal{F}_t \right] + E^Q \left[\sum_{n=1}^{NA} 1_{t_{n-1} < \tau < t_n} x(T - t_{n-1}) | \mathcal{F}_t \right] \\ &= E^Q \left[\sum_{n=1}^{NA} \left(\frac{x}{\Delta} \cdot 1_{t_{n-1} < \tau} + x(\tau - t_{n-1}) \cdot 1_{t_{n-1} < \tau < t_n} \right) | \mathcal{F}_t \right] \\ &= E^Q \left[x \int_t^{t+N} 1_{t < \tau} | \mathcal{F}_t \right] \\ &= x 1_{t < \tau} \int_t^{t+N} e^{-\int_t^s r(u) du} ds \end{aligned}$$

$$\text{And the default side: } \delta 1_{t < \tau} \int_t^{t+N} r(s) e^{-\int_t^s r(u) du} ds$$

$$\therefore \chi_t^a = \int_t^{t+N} \frac{r(s) e^{-\int_t^s r(u) du}}{e^{-\int_t^s r(u) du} ds} ds$$

$$4. \text{(a) Since } F_\theta(x_1, x_2) = (1 + e^{-x_1} + e^{-x_2} + (1-\theta)e^{-x_1-x_2})^{-1}, x_1, x_2 \in \mathbb{R}$$

$$F_{\theta,1}(x_1, \infty) = (1 + e^{-x_1})^{-1} \quad F_{\theta,2}(\infty, x_2) = (1 + e^{-x_2})^{-1}$$

which is the logistic distribution

$$\begin{aligned} \text{(b) if } \theta = 0, F_\theta(x_1, x_2) &= (1 + e^{-x_1} + e^{-x_2} + e^{-x_1-x_2})^{-1} = F_{\theta,1}(x_1) F_{\theta,2}(x_2) \\ \text{independence of } x_1, x_2 \end{aligned}$$

$$\text{(c) } F_{\theta,1}^{-1}(y) = F_{\theta,2}^{-1}(y) = -\log\left(\frac{1}{y} - 1\right)$$

$$\begin{aligned} C_0(u_1, u_2) &= F_\theta(F_{\theta,1}^{-1}(u_1), F_{\theta,2}^{-1}(u_2)) = \left(\frac{1}{u_1} + \frac{1}{u_2} - 1 + (1-\theta) \left(\frac{1}{u_1} - 1 \right) \left(\frac{1}{u_2} - 1 \right) \right)^{-1} \\ &= \frac{u_1 u_2}{u_1 + u_2 - u_1 u_2 + (1-\theta)(1-u_1)(1-u_2)} = \frac{u_1 u_2}{1-\theta(1-u_1)(1-u_2)} \end{aligned}$$